added fns_closed

theories/Spilling.v
@@ -62,13 +62,58 @@ Inductive spill_sound : nat -> (list (set var * set var)) -> (set var * set var)
   -> M_f ⊆ Sp ∪ M
     -> spill_sound k Λ (R,M) (stmtApp f Y) (ann0 (Sp,L))
 
-| SpillFun k Λ R M Sp L K s t sl_s sl_t Z
+| SpillFun k Λ R M Sp L K s t sl_s sl_t Z R_f M_f
 : cardinal (R\K ∪ L) <= k
-  -> spill_sound k (getAnn sl_s::Λ) (getAnn sl_s) s sl_s 
-  -> spill_sound k (getAnn sl_s::Λ) (R\K ∪ L, M ∪ Sp) t sl_t
+  -> cardinal R_f <= k
+  -> R_f ⊆ R\K ∪ Sp ∪ M ∪ of_list Z
+  -> M_f ⊆ R\K ∪ Sp ∪ M ∪ of_list Z
+  -> spill_sound k ((R_f,M_f)::Λ) (R_f,M_f) s sl_s 
+  -> spill_sound k ((R_f,M_f)::Λ) (R\K ∪ L, Sp ∪ M) t sl_t
     -> spill_sound k Λ (R,M) (stmtFun ((Z,s)::nil) t)
                    (annF (Sp,L) (sl_s::nil) sl_t)
 .
+
+
+Inductive spill_sound' : nat -> (list (set var * set var)) -> (set var * set var) -> stmt -> ann (set var * set var * option (set var * set var)) -> Prop :=
+
+| SpillLet' k Λ R M Sp L K Kx sl x e s
+: spill_sound' k Λ ({x;(R\K ∪ L)\Kx }, Sp ∪ M) s sl
+  -> Exp.freeVars e ⊆ R\K ∪ L
+  -> cardinal (R\K ∪ L) <= k
+  -> cardinal ({x;((R\K) ∪ L)\Kx }) <= k
+  -> spill_sound' k Λ (R,M) (stmtLet x e s) (ann1 (Sp,L,None) sl)
+
+| SpillReturn' k Λ R M Sp L K e
+: Exp.freeVars e ⊆ R\K ∪ L
+  -> cardinal ((R\K) ∪ L) <= k
+  -> spill_sound' k Λ (R,M) (stmtReturn e) (ann0 (Sp,L,None))
+
+| SpillIf' k Λ R M Sp L K sl_s sl_t e s t
+: Exp.freeVars e ⊆ R\K ∪ L
+  -> cardinal (R\K ∪ L) <= k
+  -> spill_sound' k Λ (R\K ∪ L, Sp ∪ M) s sl_s
+  -> spill_sound' k Λ (R\K ∪ L, Sp ∪ M) t sl_t
+  -> spill_sound' k Λ (R,M) (stmtIf e s t) (ann2 (Sp,L,None) sl_s sl_t)
+
+| SpillApp' k Λ R M Sp L K f Y R_f M_f
+: cardinal (R\K ∪ L) <= k
+  -> get Λ (counted f) (R_f,M_f)
+  -> R_f ⊆ R\K ∪ L
+  -> M_f ⊆ Sp ∪ M
+    -> spill_sound' k Λ (R,M) (stmtApp f Y) (ann0 (Sp,L,None))
+
+| SpillFun' k Λ R M Sp L K s t sl_s sl_t Z R_f M_f
+: cardinal (R\K ∪ L) <= k
+  -> cardinal R_f <= k
+  -> R_f ⊆ R\K ∪ Sp ∪ M ∪ of_list Z
+  -> M_f ⊆ R\K ∪ Sp ∪ M ∪ of_list Z
+  -> spill_sound' k ((R_f,M_f)::Λ) (R_f,M_f) s sl_s 
+  -> spill_sound' k ((R_f,M_f)::Λ) (R\K ∪ L, Sp ∪ M) t sl_t
+    -> spill_sound' k Λ (R,M) (stmtFun ((Z,s)::nil) t)
+                   (annF (Sp,L,Some (R_f,M_f)) (sl_s::nil) sl_t)
+.
+
+
 
 Inductive fv_e_bounded : nat -> stmt -> Prop :=
 
@@ -91,7 +136,36 @@ Inductive fv_e_bounded : nat -> stmt -> Prop :=
 : fv_e_bounded k (stmtApp f Y)
 
 | BoundFun k Z s t 
-: fv_e_bounded k (stmtFun ((Z,s)::nil) t)
+: fv_e_bounded k s
+  -> fv_e_bounded k t
+  -> fv_e_bounded k (stmtFun ((Z,s)::nil) t)
+.
+
+Inductive fns_closed : list (set var * set var) -> set var -> stmt -> Prop := 
+
+| fnsClosedLet Λ RM RM' x e s
+: RM' [=] RM
+-> fns_closed Λ {x; RM} s
+  -> fns_closed Λ RM' (stmtLet x e s)
+
+| fnsClosedReturn Λ RM e
+: fns_closed Λ RM (stmtReturn e)
+
+| fnsClosedIf Λ RM e s t
+: fns_closed Λ RM s
+-> fns_closed Λ RM t
+  -> fns_closed Λ RM (stmtIf e s t)
+
+| fnsClosedApp Λ RM f Y R_f M_f
+: get Λ (counted f) (R_f,M_f)
+  -> fns_closed Λ RM (stmtApp f Y)
+
+| fnsClosedFun Λ RM Z s t R_f M_f
+: R_f ⊆ RM
+-> M_f ⊆ RM
+-> fns_closed ((R_f,M_f)::Λ) RM s
+-> fns_closed ((R_f,M_f)::Λ) RM t
+  -> fns_closed Λ RM (stmtFun ((Z,s)::nil) t)
 .
 
 Fixpoint stupSpill (R : set var) (s : stmt) : ann (set var * set var) := 
@@ -108,9 +182,112 @@ match s with
 end.
 
 
+Fixpoint stupSpill' (R : set var) (s : stmt) (Lv : ann (set var)) : ann (set var * set var * option (set var * set var)) := 
+match s,Lv with
+| stmtLet x e t, ann1 LV lv => ann1 (R, Exp.freeVars e, None)
+                        (stupSpill' (singleton x) t lv)
+| stmtReturn e, _ => ann0 (∅, Exp.freeVars e, None)
+| stmtIf e t v, ann2 LV lv_s lv_t => ann2 (R, Exp.freeVars e, None)
+                       (stupSpill' (Exp.freeVars e) t lv_s) 
+                       (stupSpill' (Exp.freeVars e) v lv_t)
+| stmtApp f Y, _  => ann0 (R, ∅, None)
+| stmtFun ((Z,t)::nil) v, annF LV (lv_t::nil) lv_v  =>
+        annF (R, {}, Some ({}, LV)) ((stupSpill' ∅ t lv_t)::nil) 
+                                     (stupSpill' ∅ v lv_v)
+| _,_ => ann0 (∅, ∅, None)
+end.
+
+Lemma union_assoc (X Y Z : set var) : X ∪ (Y ∪ Z) [=] (X ∪ Y) ∪ Z.
+Proof.
+cset_tac.
+Qed.
+
+Lemma stupSpill_sat_spillSound (k:nat) (s:stmt) (R R' M : set var) 
+  (Λ : list (set var * set var)) (Lv : list (set var)) (ZL : list params)
+  (alv : ann (set var)) :
+k > 0
+-> R [=] R'
+-> freeVars s ⊆ R ∪ M
+-> fv_e_bounded k s
+-> live_sound Imperative ZL Lv s alv
+-> fns_closed Λ (R ∪ M) s
+(*-> getAnn alv ⊆ R' ∪ M 
+-> PIR2 (fun RMf G => fst RMf [=] ∅ /\ snd RMf [=] G) Λ (Lv \\ ZL) *)
+-> spill_sound' k Λ (R,M) s (stupSpill' R' s alv).
+
+Proof.
+intro kgeq1. revert R R' M Λ Lv ZL alv. induction s;
+  intros R R' M Λ Lv ZL alv ReqR' fvRM fvBound lvSound fClosed;
+  inversion_clear fvBound
+    as [k0 x0 e0 s0 fvBcard fvBs
+       |k0 e0 fvBcard
+       |k0 e0 s0 t0 fvBcard fvBs fvBt 
+       |k0 f0 Y0 
+       |k0 Z0 s0 t0 fvBs fvBt];
+  inversion_clear lvSound
+    as [ZL0 Lv' x' e' s' lv' al' lvS_s lvS_e lvS_al lvS_x
+       |ZL0 Lv' x' e' s1' s2' lv' al1' al2' lvS1 lvS2 lvS_e lvS_al1 lvS_al2 
+       |ZL' Lv' x' l' Y' lv' blv' Z' lvS_Z lvS_blv lvS_cnd lvS_YZ lvS_fa  
+       |ZL' Lv' x' e' lv' lvS_e 
+       | 
+       |ZL' Lv' F' t' lv' als' alb' lvS_t lvS_snd lvS_fst lvS_alb];
+  inversion_clear fClosed
+    as [Λ'' RM RM' x'' e'' s'' fCrm fCs
+       |Λ'' RM e''
+       |Λ'' RM e'' s'' t'' fCs fCt
+       |Λ'' RM f'' Y'' R_f M_f fCget
+       |Λ'' RM Z'' s'' t'' R_f M_f fCsubR fCsubM fCs fCt];
+  simpl in *. 
+
+- eapply SpillLet' with (K:= R) (Kx := Exp.freeVars e).
+  + assert (seteq : singleton x [=] {x; R\R ∪ Exp.freeVars e \ Exp.freeVars e}).
+    { cset_tac. }
+    eapply IHs; eauto with cset.
+    * rewrite seteq. reflexivity.
+    * rewrite <- seteq. rewrite <- ReqR'. rewrite <- fvRM. 
+      cset_tac. decide (x === a); eauto with cset.
+    * admit. (* how? *)
+  + cset_tac.
+  + assert (seteq : R \ R ∪ Exp.freeVars e [=] Exp.freeVars e).
+    { cset_tac. }
+    rewrite seteq. rewrite fvBcard. trivial.
+  + assert (seteq :{x; R \ R ∪ Exp.freeVars e \ Exp.freeVars e} [=] singleton x).
+    { cset_tac. }
+    rewrite seteq. rewrite singleton_cardinal. omega. 
+- eapply SpillIf' with (K:= R).
+  + cset_tac.
+  + assert (seteq : R\R ∪ Exp.freeVars e [=] Exp.freeVars e). { cset_tac. }
+    rewrite seteq. rewrite fvBcard. trivial.
+  + eapply IHs1; eauto with cset. 
+    * cset_tac.
+    * rewrite <- ReqR'. rewrite <- fvRM. cset_tac.
+    * admit. (* how? *)
+  + eapply IHs2; eauto with cset.
+    * cset_tac.
+    * rewrite <- ReqR'. rewrite <- fvRM. cset_tac.
+- (*specialize (exF l Y).
+  assert (exists R_f M_f, get Λ (labN l) (R_f, M_f)).
+          { apply exF. auto. }
+  destruct H3 as [R_f H3].
+  destruct H3 as [M_f H3].*)
+  eapply SpillApp' with (K:= R) (R_f := R_f) (M_f := M_f).
+  + assert (seteq : R \ R ∪ ∅ [=] ∅). { cset_tac. }
+    rewrite seteq. rewrite empty_cardinal. omega.
+  + eauto.
+  + admit.
+  + admit.
+- eapply SpillReturn' with (K:= R).
+  + cset_tac.
+  + assert (seteq : R\R ∪ Exp.freeVars e [=] Exp.freeVars e). { cset_tac. }
+    rewrite seteq. rewrite fvBcard. trivial.
+- destruct alv; inversion lvSound.
+  + simpl. eapply SpillFun'. simpl. admit. 
+  + simpl. eapply SpillFun' with (K:=R).
 
 
-Lemma stupSpill_sat_spillSound (k:nat) (s:stmt) (R R' M : set var) Λ Lv ZL alv :
+Lemma stupSpill_sat_spillSound (k:nat) (s:stmt) (R R' M : set var)
+      (Λ : list (set var * set var)) (Lv : list (set var)) (ZL :list params) 
+      (alv : ann (set var)) :
 k > 0
 -> freeVars s ⊆ R' ∪ M
 -> R' ⊆ R
@@ -121,8 +298,11 @@ k > 0
 -> spill_sound k Λ (R,M) s (stupSpill R' s).
 
 Proof.
-  intros knotzero subs.
-  general induction s; invt fv_e_bounded; invt live_sound; simpl in *.
+  intros knotzero subs H H0 H1 H2 H3. 
+  general induction s; invt fv_e_bounded; invt live_sound;
+ 
+ simpl in *.
+ 
    - simpl. eapply SpillLet with (K := R)(Kx := Exp.freeVars e).
      + eapply IHs; eauto.
        * rewrite <- subs. clear_all. cset_tac. decide (x === a); eauto. 
@@ -160,14 +340,49 @@ Proof.
      + assert (R \ R ∪ Exp.freeVars e [=] Exp.freeVars e).
        * cset_tac.
        * rewrite H4. auto.
-   - eapply SpillFun with (K := R); simpl in *.
+   - destruct als; [ isabsurd | destruct als; [|isabsurd] ].
+     eapply SpillFun with (K := R) (R_f := ∅) (M_f := getAnn a \ of_list Z).  
      + assert (R\R ∪ ∅ [=] ∅) as empty. 
        * clear_all. cset_tac. 
        * rewrite empty. rewrite empty_cardinal. omega.
-     + admit.
-     + admit.    
+     + (*specialize IHs with (k := k)
+                           (ZL := Z :: ZL)
+                           (Lv := getAnn ⊝ als ++ Lv)
+                           (R' := R')
+                           (R := R)
+                           (M := M)
+                           (Λ := (getAnn (stupSpill ∅ s0)) ::  Λ)
+                           (alv := alb).
+       (*rewrite <- surjective_pairing in IHs.*)
 
-Qed.
+       assert (spill_sound k ((getAnn (stupSpill ∅ s0)) ::  Λ) 
+                           (R,M) s (stupSpill R' s)).
+       apply IHs; eauto with cset.
+       * rewrite <- subs. cset_tac. 
+       * admit. 
+       * rewrite empty_cardinal. admit.*) admit.
+     + admit. 
+     + admit.
+     + admit. 
+       
+     + specialize IHs with (k:=k)
+                           (ZL := fst ⊝ ((Z, s0) :: nil) ++ ZL)
+                           (Lv := getAnn ⊝ (a :: nil) ++ Lv)
+                           (R':= ∅) 
+                           (*(R := R \ R ∪ ∅)
+                           (M :=  R' ∪ M)*)
+                          (* (Λ := (∅, (getAnn a) \ (of_list Z)) :: Λ)*)
+                           (alv := alb).
+       eapply IHs; eauto with cset.
+       rewrite <- subs. clear. cset_tac.
+       simpl. econstructor.
+       split; simpl.
+          eauto with cset.
+          cset_tac. eauto.
+          
+
+
+
 
 
 
